specs/Spec.Tree.Lemmas.fsti
@@ -417,3 +417,68 @@ val lemma_build_tree_rec:
     forest_freq ts0 hs0 == forest_freq ts2 hs2 /\
     U32.v heap_size - ts2.heap_max + ts2.heap_len == flc2 + fnc2 /\
     node + 1 == ts2.tree_len / 2 + fnc2 + 1))
+
+type symbol_index (ts: tree_state_wf) = i: nat{i < ts.tree_len / 2}
+
+/// The sum of frequencies of the symbols in the tree array.
+let rec tree_symbols_freq (ts: heap_elems_wf_ts) (i: symbol_index ts) : Tot nat =
+  if i = 0 then
+    U16.v (ts.tree.[i]).freq_or_code 
+  else
+    U16.v (ts.tree.[i]).freq_or_code + tree_symbols_freq ts (i - 1)
+
+let insert_symbols_pre (ts: heap_elems_wf_ts) (i: symbol_index ts) =
+  let tsf = tree_symbols_freq ts (ts.tree_len / 2 - 1) in
+  ts.heap_len <= i /\ ts.heap_max == U32.v heap_size /\
+  0 < tsf /\ tsf < pow2 15 /\
+  (forall j.
+    Leaf? ts.forest.[j] /\
+    id ts.forest.[j] == j /\
+    freq ts.forest.[j] == U16.v (ts.tree.[j]).freq_or_code /\
+    U16.v (ts.tree.[j]).dad_or_len == 0) /\
+  (ts.heap_len == 0 /\ i > 0 ==> tree_symbols_freq ts (i - 1) == 0) /\
+  (heap_not_empty ts ==>
+    forest_freq ts (heap_seq ts) == tree_symbols_freq ts (i - 1) /\
+    is_forest_wf ts /\
+    length (forest_symbols ts (heap_seq ts)) == length (element_seq ts) /\
+    (forall j. (forest_symbols ts (heap_seq ts)).[j] == U32.v (element_seq ts).[j]) /\
+    (forall j. mem j (heap_seq ts) ==> U32.v j < i) /\
+    (forall (j: nat{j < i}).
+      U16.v (ts.tree.[j]).freq_or_code > 0 <==>
+      mem (U32.uint_to_t j) (heap_seq ts)))
+
+let insert_symbols_post (ts: heap_elems_wf_ts) (ts': heap_elems_wf_ts) =
+  ts'.tree_len == ts.tree_len /\
+  ts.tree == ts.tree /\
+  heap_not_empty ts' /\
+  is_forest_wf ts' /\
+  (forall (j: symbol_index ts).
+    U16.v (ts'.tree.[j]).freq_or_code > 0 <==> mem (U32.uint_to_t j) (heap_seq ts'))
+
+val lemma_insert_symbols_rec: ts: heap_elems_wf_ts -> i: symbol_index ts -> Lemma
+  (requires
+    insert_symbols_pre ts i /\
+    i + 1 < ts.tree_len / 2 /\
+    U16.v (ts.tree.[i]).freq_or_code > 0)
+  (ensures (
+    let ts' = {
+      ts with
+      heap = ts.heap.(ts.heap_len + 1) <- U32.uint_to_t i;
+      heap_len = ts.heap_len + 1
+    } in
+    insert_symbols_pre ts' (i + 1)
+  ))
+
+val lemma_insert_symbols_term: ts: heap_elems_wf_ts -> i: symbol_index ts -> Lemma
+  (requires
+    insert_symbols_pre ts i /\
+    i + 1 = ts.tree_len / 2 /\
+    U16.v (ts.tree.[i]).freq_or_code > 0)
+  (ensures (
+    let ts' = {
+      ts with
+      heap = ts.heap.(ts.heap_len + 1) <- U32.uint_to_t i;
+      heap_len = ts.heap_len + 1
+    } in
+    insert_symbols_post ts ts'
+  ))
